cleanup in inversion lemmas

theories/beta.v
@@ -94,7 +94,7 @@ Proof.
 Qed.
 
 (** Notice that a -β-> b -> u⌈a⌉ -β-> u⌈b⌉
-          and  a -β+> b -> u⌈a⌉ -β+> u⌈b⌉
+            and a -β+> b -> u⌈a⌉ -β+> u⌈b⌉
     DO NOT HOLD because u might no contain
     any occurence of the variable 0 and hence,
     there would be no reduction because u⌈a⌉ = u⌈b⌉ = u⌈_⌉ *)
@@ -104,7 +104,7 @@ Proof.
   intros []; simpl; eauto.
 Qed.
 
-(** Left inversions lemmas for t -β-> _ *)
+(** We study inversions shapes for t -β-> _ *)
 
 Fact term_beta_inv u w :
     u -β-> w 
@@ -118,7 +118,6 @@ Fact term_beta_inv u w :
 Proof. intros []; simpl; eauto. Qed.
 
 (*
-
 
 Inductive term_beta_lam_invt : term -> term -> Prop :=
   | term_beta_lam_invt0 u v : u -β-> v -> term_beta_lam_invt (λ u) (λ v).
@@ -141,11 +140,18 @@ Proof. intros []; simpl; constructor; auto. Qed.
 
 *)
 
-Inductive term_beta_redex_invt f a : term -> Prop :=
-  | term_beta_redex_invt0 : term_beta_redex_invt f a (f⌈a⌉)
-  | term_beta_redex_invt1 g : f -β-> g -> term_beta_redex_invt f a (λ g @ a)
-  | term_beta_redex_invt2 b : a -β-> b -> term_beta_redex_invt f a (λ f @ b)
+Inductive term_beta_redex_shape f a : term -> Prop :=
+  | term_beta_redex_shape0 : term_beta_redex_shape f a (f⌈a⌉)
+  | term_beta_redex_shape1 g : f -β-> g -> term_beta_redex_shape f a (λ g @ a)
+  | term_beta_redex_shape2 b : a -β-> b -> term_beta_redex_shape f a (λ f @ b)
   .
+
+Fact term_beta_redex_inv f a v : λ f @ a -β-> v -> term_beta_redex_shape f a v.
+Proof.
+  intros [ (? & -> & (g & -> & ?)%term_beta_inv) 
+       | [ (? & -> & ?) | (f' & E & ->)] ]%term_beta_inv; try constructor; auto.
+  inversion E; constructor.
+Qed.
 
 Fact term_beta_redex_inv' f a v :
        λ f @ a -β-> v
@@ -153,24 +159,15 @@ Fact term_beta_redex_inv' f a v :
     \/ (exists g, v = λ g @ a /\ f -β-> g)
     \/ (exists b, v = λ f @ b /\ a -β-> b).
 Proof.
-  intros [ (? & -> & (g & -> & ?)%term_beta_inv) 
-       | [ | (f' & E & ->)] ]%term_beta_inv; eauto.
-  inversion E; subst; eauto.
-Qed.
-
-Fact term_beta_redex_inv f a v :
-       λ f @ a -β-> v -> term_beta_redex_invt f a v.
-Proof.
-  intros [ (? & -> & (g & -> & ?)%term_beta_inv) 
-       | [ (? & -> & ?) | (f' & E & ->)] ]%term_beta_inv; try constructor; auto.
-  inversion E; constructor.
+  intros H%term_beta_redex_inv.
+  destruct H; eauto.
 Qed.
 
 #[global] Reserved Notation "f '@*' l" (at level 61, left associativity).
 
 Fixpoint term_app f l : term :=
   match l with
-  | nil  => f
+  | []   => f
   | x::l => (f@x) @* l
   end
 where "f @* l" := (term_app f l).
@@ -190,31 +187,17 @@ Qed.
 
 #[local] Hint Resolve term_beta_app : core.
 
+Fact term_beta_app_middle a l u v r : u -β-> v -> a @* l++u::r -β-> a @* l++v::r.
+Proof. intro; rewrite !term_app_comp; simpl; auto. Qed.
+
 Fact term_betastar_app u v l : u -β*> v -> u @* l -β*> v @* l.
 Proof. apply clos_refl_trans_fun with (f := fun u => u @* l); eauto. Qed.
 
-Fact term_beta_app_middle a l u v r : 
-        u -β-> v -> a @* l++u::r -β-> a @* l++v::r.
-Proof. intro; rewrite !term_app_comp; simpl; auto. Qed.
-
-Inductive term_beta_var_app_invt x : list term -> term -> Prop :=
-  | term_beta_var_app_invt0 l v w r : v -β-> w -> term_beta_var_app_invt x (l++v::r) (£x @* l++w::r).
-
-Fact term_var_app_beta_inv x m u : £x @* m -β-> u -> term_beta_var_app_invt x m u.
-Proof.
-  induction m as [ | m v IHm ] in u |- * using list_snoc_rect.
-  + intros []%term_beta_inv.
-  + rewrite term_app_snoc.
-    intros [ (a & -> & H1%IHm) 
-         | [ (a & -> & H1)
-           | (a & H1 & H2) ]]%term_beta_inv.
-    * induction H1.
-      rewrite <- term_app_snoc, !app_ass; now constructor.
-    * rewrite <- term_app_snoc.
-      now constructor 1 with (r := []).
-    * now destruct m using list_snoc_rect; 
-        [ | rewrite term_app_snoc in H1 ].
-Qed.
+(** We study the successors of _ @* _ for the following forms
+     - £_ @* _
+     - _@_ @* _
+     - λ_ @* []
+     - λ_ @* _::_ *)
 
 Definition term_neutral (u : term) :=
   match u with 
@@ -226,7 +209,8 @@ Inductive term_beta_neutral_app_invt a : list term -> term -> Prop :=
   | term_beta_neutral_app_invt0 b m : a -β-> b -> term_beta_neutral_app_invt a m (b @* m)
   | term_beta_neutral_app_invt1 l v w r : v -β-> w -> term_beta_neutral_app_invt a (l++v::r) (a @* l++w::r).
 
-Fact term_beta_neutral_app_inv a u m : 
+(** This is a key lemma for the results below, by snoc induction on m *)
+Lemma term_beta_neutral_app_inv a u m : 
         term_neutral a -> a @* m -β-> u -> term_beta_neutral_app_invt a m u.
 Proof.
   induction m as [ | m b IHm ] in a, u |- * using list_snoc_rect; intros H1 H2.
@@ -236,7 +220,7 @@ Proof.
       as [ (u' & -> & H2%IHm) 
        | [ (b' & -> & H2)
          | (k  & E & _) ] ]; auto.
-    * induction H2 as [ b' m H2 | l v w r H2 ]; rewrite <- term_app_snoc.
+    * destruct H2 as [ b' m H2 | l v w r H2 ]; rewrite <- term_app_snoc.
       - now constructor 1.
       - rewrite !app_ass; now constructor 2.
     * rewrite <- term_app_snoc.
@@ -246,20 +230,49 @@ Proof.
         now subst.
 Qed.
 
-Inductive term_beta_app_invt a b : list term -> term -> Prop :=
-  | term_beta_app_invt0 m t : a@b -β-> t -> term_beta_app_invt a b m (t @* m)
-  | term_beta_app_invt1 l v w r : v -β-> w -> term_beta_app_invt a b (l++v::r) (a @* b::l++w::r).
+Inductive term_beta_var_app_shape x : list term -> term -> Prop :=
+  | term_beta_var_app_shape0 l v w r : v -β-> w -> term_beta_var_app_shape x (l++v::r) (£x @* l++w::r).
 
-Fact term_beta_app_inv a b m u : a @* b::m -β-> u -> term_beta_app_invt a b m u.
+Fact term_beta_var_app_inv x m u : £x @* m -β-> u -> term_beta_var_app_shape x m u.
 Proof.
-  simpl; intros H%term_beta_neutral_app_inv; simpl; auto.
-  induction H; constructor; auto.
+  intros H%term_beta_neutral_app_inv; simpl; auto.
+  destruct H as [ _ _ []%term_beta_inv | ].
+  now constructor.
 Qed.
+
+Inductive term_beta_ap_app_shape a b : list term -> term -> Prop :=
+  | term_beta_ap_app_shape0 m t : a@b -β-> t -> term_beta_ap_app_shape a b m (t @* m)
+  | term_beta_ap_app_shape1 l v w r : v -β-> w -> term_beta_ap_app_shape a b (l++v::r) ((a@b) @* l++w::r).
+
+Fact term_beta_ap_app_inv a b m u : (a@b) @* m -β-> u -> term_beta_ap_app_shape a b m u.
+Proof.
+  intros H%term_beta_neutral_app_inv; simpl; auto.
+  destruct H; constructor; auto.
+Qed.
+
+Fact term_beta_lam_app0_inv a u : λ a @* [] -β-> u -> exists b, u = λ b @* [] /\ a -β-> b.
+Proof. now intros H%term_beta_inv. Qed.
+
+Inductive term_beta_redex_app_shape u a : list term -> term -> Prop :=
+  | term_beta_redex_app_shape0 m : term_beta_redex_app_shape u a m (u⌈a⌉ @* m)
+  | term_beta_redex_app_shape1 m v : u -β-> v -> term_beta_redex_app_shape u a m (λ v @* a::m)
+  | term_beta_redex_app_shape2 m b : a -β-> b -> term_beta_redex_app_shape u a m (λ u @* b::m)
+  | term_beta_redex_app_shape3 l v w r : v -β-> w -> term_beta_redex_app_shape u a (l++v::r) (λ u @* a::l++w::r).
+
+Fact term_beta_redex_app_inv u a m t : λ u @* a::m -β-> t -> term_beta_redex_app_shape u a m t.
+Proof.
+  intros H%term_beta_ap_app_inv.
+  destruct H as [ m t H%term_beta_redex_inv | ].
+  + destruct H; now constructor.
+  + now constructor.
+Qed.
+
+(** We study strong normalization *)
 
 Definition term_beta_normal u := forall v, ~ u -β-> v.
 
 Fact term_var_beta_normal x : term_beta_normal (£x).
-Proof. now intros v ?%term_beta_inv. Qed.
+Proof. now intros ? ?%term_beta_inv. Qed.
 
 Definition term_beta_sn := Acc (fun u v => term_beta v u).
 
@@ -292,21 +305,6 @@ Qed.
        term_betastar_app term_betastar_replace
      term_beta_app_middle : core.
 
-Inductive term_beta_abs_app_invt u a : list term -> term -> Prop :=
-  | term_beta_abs_app_invt0 m : term_beta_abs_app_invt u a m (u⌈a⌉ @* m)
-  | term_beta_abs_app_invt1 m v : u -β-> v -> term_beta_abs_app_invt u a m (λ v @* a::m)
-  | term_beta_abs_app_invt2 m b : a -β-> b -> term_beta_abs_app_invt u a m (λ u @* b::m)
-  | term_beta_abs_app_invt3 l v w r : v -β-> w -> term_beta_abs_app_invt u a (l++v::r) (λ u @* a::l++w::r).
-
-Proposition term_beta_abs_app_inv u a m t :
-          λ u @* a::m -β-> t -> term_beta_abs_app_invt u a m t.
-Proof.
-  intros H%term_beta_app_inv.
-  induction H as [ m t H%term_beta_redex_inv | ].
-  + induction H; now constructor.
-  + now constructor.
-Qed.
-
 (** This proof DOES NOT require computing the SN height of a and u⌈a⌉@*l 
      which gives a MAJOR SIMPLIFICATION over the previous version in the 
      coq-terms project, and also departs from the proof in Krivine's book *)
@@ -320,18 +318,19 @@ Proof.
   fold SN;
   intros a u m H1 H2 IH1 IH2.
 
-  (** Now we can proceed with the proof with the proper IH
-      First the Acc constructor and then case analysis on the
-      possible successors of λu @* a::m which are, according
-      to term_beta_abs_app_inv
+  (** Now we can proceed with the proof.
+      First the Acc constructor and 
+      then case analysis on the
+      possible successors of λu @* a::m 
+      given by term_beta_redex_app_inv:
         + u⌈a⌉ @* m                  (Hm works)
         + λv @* a::m with u -β-> v   (IH2 works)
         + λu @* b::m with a -β-> b   (IH1 works)
         + λu @* a::m' with m -β-> m'
              at one position in m    (IH2 works)
     *)
-  constructor; fold SN; intros t H%term_beta_abs_app_inv.
-  induction H as [ m | m v Hv | m b Hb | l v w r Hv ].
+  constructor; fold SN; intros ? H%term_beta_redex_app_inv.
+  destruct H as [ m | m v Hv | m b Hb | l v w r Hv ].
   + (** SN (u⌈a⌉ @* m) *)
     trivial.
   + (** SN ((λv)@a @* m) *)
